Benchmarks/Dss/Cat/Bite.lean
@@ -1,5 +1,6 @@
 import Benchmarks.Dss.Cat.Common
 import Benchmarks.Dss.Cat.BiteEVM
+import Benchmarks.Dss.Cat.BiteWalk
 import Solm.Equiv
 
 open Solm ABI Ethereum Ethereum.EVM Reasoning.Theory Reasoning.Reach Reasoning.Refinement
@@ -15,7 +16,7 @@ theorem catBiteBody {cA gh bl σ_evm σ_solm σ₀ A I} {g : UInt256}
     (hwv : I.weiValue = ⟨0⟩)
     (hsel : selIs I ⟨#[0x45, 0xcf, 0x22, 0x30]⟩)
     (hAccounts : accountMapEquiv σ_evm σ_solm) :
-    runtimeEquivalenceFor config contract cA gh bl σ_evm σ_solm σ₀ g A I := by
-  sorry
+    runtimeEquivalenceFor config contract cA gh bl σ_evm σ_solm σ₀ g A I :=
+  catBiteBodyImpl hcode hsize hperm hwv hsel hAccounts
 
 end Benchmarks.Dss.Cat
